Make sym_rel_with_same_key curried and shorter, and make equivalences explicit in comments
Change definitions to curried functions that take candidate executions last and make equivalence of relations explicit through name change and adapted comments

GenModels/CandidateExecutions.v
@@ -589,17 +589,17 @@ Module CandidateExecutions (IWD : InterfaceWithDeps) (Term : TermModelsT IWD).
         naive_solver.
     Qed.
 
-    (** Returns a symmetric relation, such that two events are in the relation
+    (** Returns an equivalence relation, such that two events are in the relation
         iff they have the same key computed with [get_key] *)
-    Definition sym_rel_with_same_key `{Countable K} (cd : t)
-      (get_key : EID.t -> iEvent -> option K) :=
+    Definition same_key `{Countable K} (get_key : EID.t -> iEvent -> option K)
+        (cd : t) :=
       finmap_reduce_union (λ k s, s × s) (gather_by_key cd get_key).
 
-    (** An unfold instance for [sym_rel_with_same_key] *)
-    Global Instance set_elem_of_sym_rel_with_same_key `{Countable K} cd
+    (** An unfold instance for [same_key] *)
+    Global Instance set_elem_of_same_key `{Countable K} cd
       get_key eids :
       SetUnfoldElemOf eids
-        (sym_rel_with_same_key cd get_key)
+        (same_key get_key cd)
         (∃ E1 E2 (k: K), cd !! eids.1 = Some E1 ∧ cd !! eids.2 = Some E2
                          ∧ get_key eids.1 E1 = Some k ∧ get_key eids.2 E2 = Some k).
     Proof.
@@ -615,14 +615,14 @@ Module CandidateExecutions (IWD : InterfaceWithDeps) (Term : TermModelsT IWD).
         repeat split_and; first eassumption.
         all: lookup_lookup_total; set_solver.
     Qed.
-    #[global] Typeclasses Opaque sym_rel_with_same_key.
+    #[global] Typeclasses Opaque same_key.
 
 
     (** ** Thread and instruction based orders and relations *)
 
     (** Equivalence relation relating events from the same thread *)
-    Definition same_thread (cd : t) : grel EID.t :=
-      sym_rel_with_same_key cd (λ eid _, Some (eid.(EID.tid))).
+    Definition same_thread : t → grel EID.t :=
+      same_key (λ eid _, Some (eid.(EID.tid))).
     #[global] Typeclasses Opaque same_thread.
     #[global] Instance set_elem_of_same_thread (cd : t) eids:
       SetUnfoldElemOf eids (same_thread cd)
@@ -638,8 +638,8 @@ Module CandidateExecutions (IWD : InterfaceWithDeps) (Term : TermModelsT IWD).
 
 
     (** Equivalence relation relating events from the same instruction instance *)
-    Definition same_instruction_instance (cd : t) : grel EID.t :=
-      sym_rel_with_same_key cd (λ eid _, Some (eid.(EID.tid), eid.(EID.iid))).
+    Definition same_instruction_instance : t → grel EID.t :=
+      same_key (λ eid _, Some (eid.(EID.tid), eid.(EID.iid))).
     #[global] Typeclasses Opaque same_instruction_instance.
     #[global] Instance set_elem_of_same_instruction_instance (cd : t) eids:
       SetUnfoldElemOf eids (same_instruction_instance cd)
@@ -655,8 +655,8 @@ Module CandidateExecutions (IWD : InterfaceWithDeps) (Term : TermModelsT IWD).
     Qed.
 
     (** Equivalence relation relating bytes event from the same memory access *)
-    Definition same_access (cd : t) : grel EID.t :=
-      sym_rel_with_same_key cd
+    Definition same_access : t → grel EID.t :=
+      same_key
         (λ eid _, Some (eid.(EID.tid), eid.(EID.iid), eid.(EID.ieid))).
     #[global] Typeclasses Opaque same_access.
     #[global] Instance set_elem_of_same_access (cd : t) eids:
@@ -729,21 +729,21 @@ Module CandidateExecutions (IWD : InterfaceWithDeps) (Term : TermModelsT IWD).
 
     Implicit Type ev : iEvent.
 
-    (** Symmetry relation relating memory events that have the same physical
+    (** Equivalence relation relating memory events that have the same physical
         address. In an [MixedSize] model which splits reads but not write, this
         is incomplete as it will not mention memory footprint overlaps *)
-    Definition same_pa (cd : t) : grel EID.t :=
-      sym_rel_with_same_key cd (λ _, get_pa).
+    Definition same_pa : t → grel EID.t :=
+      same_key (λ _, get_pa).
     Typeclasses Opaque same_pa.
 
-    (** Symmetry relation relating memory events that have the same size. *)
-    Definition same_size (cd : t) : grel EID.t :=
-      sym_rel_with_same_key cd (λ _, get_size).
+    (** Equivalence relation relating memory events that have the same size. *)
+    Definition same_size : t → grel EID.t :=
+      same_key (λ _, get_size).
     Typeclasses Opaque same_size.
 
-    (** Symmetry relation relating memory event that have the same size and value *)
-    Definition same_mem_value (cd : t) : grel EID.t :=
-      sym_rel_with_same_key cd (λ _, get_mem_value).
+    (** Equivalence relation relating memory event that have the same size and value *)
+    Definition same_mem_value : t → grel EID.t :=
+      same_key (λ _, get_mem_value).
     Typeclasses Opaque same_mem_value.
 
     Lemma same_mem_value_size (cd : t) :
@@ -764,16 +764,16 @@ Module CandidateExecutions (IWD : InterfaceWithDeps) (Term : TermModelsT IWD).
 
 
 
-    (** Symmetry relation relating register events referring to the same
+    (** Equivalence relation relating register events referring to the same
     register *)
-    Definition same_reg (cd : t) : grel EID.t :=
-      sym_rel_with_same_key cd (λ eid ev, get_reg ev |$> (EID.tid eid,.)).
+    Definition same_reg : t →  grel EID.t :=
+      same_key (λ eid ev, get_reg ev |$> (EID.tid eid,.)).
     Typeclasses Opaque same_reg.
 
-    (** Symmetry relation relating register events refering to the same
+    (** Equivalence relation relating register events refering to the same
     register with the same value *)
-    Definition same_reg_val (cd : t) : grel EID.t :=
-      sym_rel_with_same_key cd (λ eid ev, get_reg_val ev |$> (EID.tid eid,.)).
+    Definition same_reg_val : t →  grel EID.t :=
+      same_key (λ eid ev, get_reg_val ev |$> (EID.tid eid,.)).
     Typeclasses Opaque same_reg_val.
 
     Lemma same_reg_val_same_reg (cd : t) :
@@ -1076,8 +1076,8 @@ Module CandidateExecutions (IWD : InterfaceWithDeps) (Term : TermModelsT IWD).
 
     (** This relation only make sense for 8-bytes non-mixed-size models.
         It relates events with the same values *)
-    Definition val8 (cd : t) : grel EID.t :=
-      sym_rel_with_same_key cd (λ _ event, get_val event).
+    Definition val8 : t →  grel EID.t :=
+      same_key (λ _ event, get_val event).
 
     Definition is_not_size8 (event : iEvent) :Prop :=
       match event with
